practice.v
@@ -2,6 +2,7 @@ Require Import Coq.Arith.Arith.
 Require Import Coq.Arith.PeanoNat.
 Require Import Coq.Arith.Even.
 
+Require Import AbstractBool.
 Require Import AbstractState.
 Require Import AbstractInterpreter.
 Require Import Aux.
@@ -35,7 +36,6 @@ Lemma abstract_aexp_var_sound : forall x,
 Proof. intros. unfold sound_aexp. intros. simpl. unfold sound_state in H.
   apply H. Qed.
 
-
 Theorem abstract_aexp_eval_sound : forall e,
   sound_aexp e.
 Proof. 
@@ -44,6 +44,37 @@ Proof.
   - (* AVar *) apply abstract_aexp_var_sound. 
   - (* APlus *) apply abstract_aexp_plus_sound; auto.
   - (* AMult *) apply abstract_aexp_mult_sound; auto.
+Qed.
+
+Lemma abstract_beval_eq_sound : forall a1 a2,
+  sound_bexp (BEq a1 a2).
+Proof.
+  unfold sound_bexp. intros. simpl. pose proof abstract_aexp_eval_sound. 
+  unfold sound_aexp in H0. assert (sound_par (abstract_eval_aexp ast a1)
+  (eval_aexp st a1)).
+  { apply H0. assumption. }
+  assert (sound_par (abstract_eval_aexp ast a2) (eval_aexp st a2)).
+  { apply H0. assumption. }
+  clear H0. 
+  destruct (abstract_eval_aexp ast a1) eqn:Ha1; 
+  destruct (abstract_eval_aexp ast a2) eqn:Ha2; try reflexivity; simpl in *.
+  - destruct (Nat.eqb (eval_aexp st a1) (eval_aexp st a2)) eqn:Heq; 
+    try reflexivity.
+    pose proof not_even_and_odd. apply Nat.eqb_eq in Heq. rewrite Heq in H1.
+    simpl. apply H0 with (n:=(eval_aexp st a2)); assumption.
+  - destruct (Nat.eqb (eval_aexp st a1) (eval_aexp st a2)) eqn:Heq;
+    try reflexivity.
+    pose proof not_even_and_odd. apply Nat.eqb_eq in Heq. rewrite Heq in H1.
+    simpl. apply H0 with (n:=(eval_aexp st a2)); assumption.
+Qed.
+
+Theorem abstract_beval_sound : forall e,
+  sound_bexp e.
+Proof. 
+  unfold sound_bexp. intros. induction e; try reflexivity.
+  - apply abstract_beval_eq_sound. assumption. 
+  - simpl. apply neg_ab_sound. assumption.
+  - simpl. apply and_ab_sound. assumption. assumption.
 Qed.
 
 Lemma abstract_ceval_ass_sound : forall y a,
